geb-lean/GebLean/LawvereNatBTBackTrans.lean
@@ -45,6 +45,7 @@ def NatBTMor1.isFoldFree : {nm : ℕ × ℕ} → {σ : NatBTSort} →
       nm'.2 = 0 ∧ f.isFoldFree ∧ ∀ i, (gNat i).isFoldFree
   | _, _, NatBTMor1.foldBTNat _ _ _ _ => False
   | _, _, NatBTMor1.foldBTBT _ _ _ _ => False
+  | _, _, NatBTMor1.boundedNatRec _ _ _ _ => False
   | _, _, NatBTMor1.encodeBT t => t.isFoldFree
   | _, _, NatBTMor1.decodeBT k => k.isFoldFree
 
@@ -93,6 +94,7 @@ def NatBTMor1.toERUniform : {nm : ℕ × ℕ} → {σ : NatBTSort} →
       else
         ERMor1.zeroN _
   | _, _, NatBTMor1.foldBTBT _ _ _ _ => ERMor1.zeroN _
+  | _, _, NatBTMor1.boundedNatRec _ _ _ _ => ERMor1.zeroN _
   | _, _, NatBTMor1.decodeBT k => k.toERUniform
 
 /-- Back-translation specialized to `.nat` outputs. -/
@@ -289,6 +291,10 @@ theorem NatBTMor1.toERUniform_interp_aux :
       exact absurd h (by
         simp [NatBTMor1.isFoldFree])
   | foldBTBT _ _ _ _ _ _ _ _ =>
+      intro h _ _
+      exact absurd h (by
+        simp [NatBTMor1.isFoldFree])
+  | boundedNatRec _ _ _ _ _ _ _ _ =>
       intro h _ _
       exact absurd h (by
         simp [NatBTMor1.isFoldFree])
